GraphAlg/algorithms/test_floyd.v
@@ -1,0 +1,2 @@
+Require Import GraphLib.examples.floyd.
+Check floyd_relaxation_correct.
